Examples/Ring/RingAbs.lean
@@ -42,7 +42,10 @@ invariant [leader_greatest] leader L → le N L
 invariant [self_msg_greatest] pending L L → le N L
 invariant [drop_smaller] pending S D ∧ btw S N D → le N S
 
-#time #gen_spec
+set_option veil.solver "smt"
+set_option veil.smt.trust false
+
+#gen_spec
 
 #model_check { node := Fin 4 } { }
 
